\documentclass{article}
\usepackage[fleqn]{mathtools}
\usepackage{xfrac}
\begin{document}
\begin{equation}
F = C\bigg(\frac{r_+b_+-sa_+}{a_+^2+b_+^2}+\frac{r_-b_--sa_-}{a_-^2+b_-^2}\bigg)
\end{equation}
\begin{equation}
a_\pm = 4\pi^2(\nu_o-\nu\pm J/2)^2-(\tau^{-1}+\tau_2^{-1})^2-\pi^2(\nu_1-\nu_2)^2-\pi^2 J^2 + \tau^{-2}
\end{equation}
\begin{equation}
b_\pm = 4\pi(\nu_o-\nu\pm J/2)(\tau^{-1}+\tau_2^{-1})\mp 2\pi J\tau^{-1}
\end{equation}
\begin{equation}
r_\pm = 2\pi(\nu_o-\nu\pm J)
\end{equation}
\begin{equation}
s = 2\tau^{-1}+\tau_2^{-1}
\end{equation}
\begin{equation}
\nu_o = \frac{\nu_1 + \nu_2)}{2}
\end{equation}
\begin{equation}
\tau = k^{-1}
\end{equation}
\begin{equation}
\tau_2 = \frac{1}{\pi W_{\sfrac{1}{2}}}
\end{equation}

\end{document}